src/ShouldBuild.v
@@ -59,8 +59,8 @@ From Perennial.program_proof.simplepb Require
 
 From Perennial.program_proof.simplepb.simplelog Require proof.
 
-From Perennial.program_proof.simplepb.apps Require kv_proof closed_wpcs.
-(* closed_proof . *)
+From Perennial.program_proof.simplepb.apps Require kv_proof.
+     (* closed_wpcs closed_proof . *)
 
 From Perennial.program_proof.mpaxos Require
      applyasfollower_proof.
