src/program_proof/simplepb/pb_increasecommit_proof.v
@@ -10,14 +10,13 @@ Import RecordSetNotations.
 
 Section pb_increasecommit_proof.
 Context `{!heapGS Σ}.
-Context {pb_record:Sm.t}.
+Context {params:pbParams.t}.
+Import pbParams.
 
 Notation OpType := (Sm.OpType pb_record).
 Notation has_op_encoding := (Sm.has_op_encoding pb_record).
 Notation has_snap_encoding := (Sm.has_snap_encoding pb_record).
 Notation compute_reply := (Sm.compute_reply pb_record).
-Notation pbG := (pbG (pb_record:=pb_record)).
-Notation own_Server_ghost_f := (own_Server_ghost_f (pb_record:=pb_record)).
 
 Context `{!waitgroupG Σ}.
 Context `{!pbG Σ}.
