src/program_proof/simplepb/pb_leaserenewal_proof.v
@@ -13,19 +13,18 @@ Import RecordSetNotations.
 Section pb_leaserenewal_proof.
 
 Context `{!heapGS Σ}.
-Context {pb_record:Sm.t}.
+Context {params:pbParams.t}.
+Import pbParams.
+
 Notation OpType := (pb_record.(Sm.OpType)).
 Notation has_op_encoding := (Sm.has_op_encoding pb_record).
 Notation has_snap_encoding := (Sm.has_snap_encoding pb_record).
 Notation compute_reply := (Sm.compute_reply pb_record).
-Notation "server.t" := (server.t (pb_record:=pb_record)).
-Notation pbG := (pbG (pb_record:=pb_record)).
-Notation get_rwops := (get_rwops (pb_record:=pb_record)).
 
 Context `{!pbG Σ}.
 
+Existing Instance toConfigParams.
 Lemma lease_renewal_step γ γsrv γconf γl newLeaseExpiration st :
-  let pNtop := (configParams.Ntop.mk $ pbN .@ "config") in
   is_lease config_proof.epochLeaseN γl (own_latest_epoch γconf st.(server.epoch)) -∗
   is_lease_valid_lb γl newLeaseExpiration -∗
   is_conf_inv γ γconf -∗
