src/program_proof/simplepb/pb_start_proof.v
@@ -11,18 +11,12 @@ From iris.algebra Require Import mono_list.
 
 Section pb_start_proof.
 
-Context {pb_record:Sm.t}.
-Notation pbG := (pbG (pb_record:=pb_record)).
+Context {params:pbParams.t}.
+Import pbParams.
 Notation OpType := (Sm.OpType pb_record).
 Notation has_op_encoding := (Sm.has_op_encoding pb_record).
 Notation has_snap_encoding := (Sm.has_snap_encoding pb_record).
 Notation compute_reply := (Sm.compute_reply pb_record).
-
-Notation wp_Clerk__ApplyAsBackup := (wp_Clerk__ApplyAsBackup (pb_record:=pb_record)).
-Notation wp_Clerk__SetState := (wp_Clerk__SetState (pb_record:=pb_record)).
-Notation wp_Clerk__GetState := (wp_Clerk__GetState (pb_record:=pb_record)).
-Notation wp_Clerk__BecomePrimary := (wp_Clerk__BecomePrimary (pb_record:=pb_record)).
-Notation wp_Clerk__Apply := (wp_Clerk__Apply (pb_record:=pb_record)).
 
 Context `{!heapGS Σ}.
 Context `{!pbG Σ}.
@@ -147,7 +141,7 @@ Proof.
   iSplitL.
   {
     repeat iExists _.
-    instantiate (1:=(server.mkC pb_record _ _ _ _ _ _ _ _)).
+    instantiate (1:=(server.mkC _ _ _ _ _ _ _ _ _)).
     simpl.
     iFrame "∗".
     iSplitL "nextIndex".
